inhale_rel field access predicate progress

InhaleRel.thy
@@ -137,25 +137,43 @@ qed
 
 subsection \<open>Field access predicate rule\<close>
 
+(*
+definition inhale_fieldacc_subexps_wf_rel
+  where "inhale_fieldacc_subexps_wf_rel e_r e_p \<equiv>       
+       (ctxt, R, Some \<omega> \<turnstile> \<langle>e_r; \<omega>\<rangle> [\<Down>]\<^sub>t Val (VRef r) \<and>
+        ctxt, R, Some \<omega> \<turnstile> \<langle>e_p; \<omega>\<rangle> [\<Down>]\<^sub>t Val (VPerm p)) \<longrightarrow>
+       W' = (if r = Null then {\<omega>} else inhale_perm_single R \<omega> (the_address r,f) (Some (Abs_prat p))) \<and>
+       th_result_rel (p \<ge> 0) (W' \<noteq> {} \<and> (p > 0 \<longrightarrow> r \<noteq> Null)) W' res"
+*)
+
 lemma inhale_rel_field_acc:
   assumes 
     MaskUpdWf: "mask_update_wf TyRep ctxt mask_upd_bpl" and
     WfRcv: "expr_wf_rel (state_rel_ext R) ctxt_vpr StateCons P ctxt e_rcv_vpr \<gamma> \<gamma>1" and
     WfPerm: "expr_wf_rel (state_rel_ext R) ctxt_vpr StateCons P ctxt e_p \<gamma>1 \<gamma>2" and
-    WfInh:  "wf_rel (state_rel_ext R)
-                  Rext' 
-                  (\<lambda> \<omega>def \<omega>. \<exists>p r. ctxt_vpr, StateCons, Some \<omega>def \<turnstile> \<langle>e_p;\<omega>\<rangle> [\<Down>]\<^sub>t (Val (VPerm p)) \<and> p \<ge> 0 \<and>
-                                   ctxt_vpr, StateCons, Some \<omega>def \<turnstile> \<langle>e_rcv_vpr;\<omega>\<rangle> [\<Down>]\<^sub>t (Val (VRef r)) \<and> (p > 0 \<longrightarrow> r \<noteq> Null))  
-                  (\<lambda> \<omega>def \<omega>. \<exists>p. ctxt_vpr, StateCons, Some \<omega>def \<turnstile> \<langle>e_p;\<omega>\<rangle> [\<Down>]\<^sub>t (Val (VPerm p)) \<and> p < 0)
+  
+    (* alternative 1 *)
+    PosPermRel:  "rel_general R
+                  R'
+                  (\<lambda> \<omega> \<omega>'. \<omega> = \<omega>' \<and> (\<exists>p. ctxt_vpr, StateCons, Some \<omega> \<turnstile> \<langle>e_p;\<omega>\<rangle> [\<Down>]\<^sub>t (Val (VPerm p)) \<and> p \<ge> 0))
+                  (\<lambda> \<omega>. (\<exists>p. ctxt_vpr, StateCons, Some \<omega> \<turnstile> \<langle>e_p;\<omega>\<rangle> [\<Down>]\<^sub>t (Val (VPerm p)) \<and> p < 0))
                   P ctxt \<gamma>2 \<gamma>3" and
-            "m_bpl = mask_var Tr" and
-    MaskUpdBpl:
-       "\<And> \<omega> ns. Rext' \<omega> \<omega> ns \<Longrightarrow> \<exists> ns'. red_ast_bpl P ctxt (\<gamma>, Normal ns) (\<gamma>', Normal ns')" and
+    UpdInhRel: "rel_general R' R
+                  (\<lambda> \<omega> \<omega>'. red_inhale ctxt_vpr StateCons (Atomic (Acc e_rcv_vpr f (PureExp e_p))) \<omega> (RNormal \<omega>'))
+                  (\<lambda> \<omega>. False) P ctxt \<gamma>3 \<gamma>'"                                  
+    (* alternative 1 finished *)
+
+    (* alternative 2 *)
+ (*   MaskUpdBpl: "rel_general R' R (\<lambda> \<omega> \<omega>'. red_inhale ctxt_vpr StateCons (Atomic (Acc e_rcv_vpr f (PureExp e_p))) \<omega> (RNormal \<omega>'))
+                                  (\<lambda> \<omega>. \<exists>p. ctxt_vpr, StateCons, Some \<omega> \<turnstile> \<langle>e_p;\<omega>\<rangle> [\<Down>]\<^sub>t (Val (VPerm p)) \<and> p < 0)  P ctxt \<gamma>2 \<gamma>3" and*)
+    (* alternative 2 finished *)
+(*
+    "m_bpl = mask_var Tr" and
     HeapUpdateBpl: "m_upd_bpl = mask_upd_bpl (Lang.Var m_bpl) e_rcv_bpl e_f_bpl new_perm_bpl [TConSingle (TNormalFieldId TyRep), \<tau>_bpl]" and    
     RcvRel: "exp_rel_vpr_bpl Rext' ctxt_vpr ctxt e_rcv_vpr rcv_bpl" and
     FieldRelSingle: "field_rel_single (program_total ctxt_vpr) TyRep Tr f_vpr e_f_bpl \<tau>_bpl" and
     NewPermRel: "exp_rel_vpr_bpl Rext' ctxt_vpr ctxt (ViperLang.Binop (Perm e_rcv_vpr f) ViperLang.Add e_p) new_perm_bpl" 
-
+*)
     (*
      \<comment>\<open>Inhale property for R\<close>
     RInhale:  "\<And> \<omega> ns ty_vpr hb r f_bpl p. Rext' \<omega> \<omega> ns \<Longrightarrow>
@@ -182,28 +200,53 @@ proof (rule inhale_rel_intro_2)
   hence Rext0: "state_rel_ext R \<omega> \<omega> ns"
     by simp
 
-  assume "red_inhale ctxt_vpr StateCons (Atomic (Acc e_rcv_vpr f (PureExp e_p))) \<omega> res"
+  assume RedInh: "red_inhale ctxt_vpr StateCons (Atomic (Acc e_rcv_vpr f (PureExp e_p))) \<omega> res"
   thus "inhale_rel_aux R ctxt_vpr StateCons P ctxt (Atomic (Acc e_rcv_vpr f (PureExp e_p))) \<gamma> \<gamma>' \<omega> ns res"
   proof (cases)
     case (InhAcc r p W')
     from this obtain ns1 where Rext1: "state_rel_ext R \<omega> \<omega> ns1" and "red_ast_bpl P ctxt (\<gamma>, Normal ns) (\<gamma>1, Normal ns1)"
       using wf_rel_normal_elim[OF WfRcv Rext0]
       by blast
-    with InhAcc obtain ns2 where Rext2: "state_rel_ext R \<omega> \<omega> ns2" and Red2: "red_ast_bpl P ctxt (\<gamma>, Normal ns) (\<gamma>2, Normal ns2)"
+    with InhAcc obtain ns2 where "state_rel_ext R \<omega> \<omega> ns2" and Red2: "red_ast_bpl P ctxt (\<gamma>, Normal ns) (\<gamma>2, Normal ns2)"
       using wf_rel_normal_elim[OF WfPerm Rext1] red_ast_bpl_transitive
       by blast
+    hence "R \<omega> ns2"
+      by simp
 
     show ?thesis
     proof (rule inhale_rel_aux_intro)
       \<comment>\<open>Normal case\<close>
-      let ?\<gamma>3 = "((BigBlock name ((Lang.Assign m_bpl m_upd_bpl)#cs) str tr), cont)"
-
+      
       fix \<omega>'
       assume "res = RNormal \<omega>'"
       hence "0 \<le> p" and "W' \<noteq> {}" and "0 < p \<longrightarrow> r \<noteq> Null" and "\<omega>' \<in> W'"
       using th_result_rel_normal InhAcc
-      by auto
+      by blast+
 
+      with InhAcc obtain ns3 where "red_ast_bpl P ctxt (\<gamma>, Normal ns) (\<gamma>3, Normal ns3)" and "R' \<omega> ns3" 
+        using rel_success_elim[OF PosPermRel \<open>R \<omega> ns2\<close>] Red2 red_ast_bpl_transitive
+        by blast
+
+      thus "\<exists>ns'. red_ast_bpl P ctxt (\<gamma>, Normal ns) (\<gamma>', Normal ns') \<and> R \<omega>' ns'"
+        using rel_success_elim[OF UpdInhRel] RedInh \<open>res = _\<close> red_ast_bpl_transitive
+        by blast
+    next
+      \<comment>\<open>Failure case\<close>
+      assume "res = RFailure"
+      hence "p < 0"
+        using th_result_rel_failure_2 InhAcc
+        by fastforce
+
+      with InhAcc show "\<exists>c'. red_ast_bpl P ctxt (\<gamma>, Normal ns) c' \<and> snd c' = Failure"
+        using rel_failure_elim[OF PosPermRel \<open>R \<omega> ns2\<close>] Red2 red_ast_bpl_transitive
+        by blast
+    qed
+
+        
+   
+      
+        
+     (*
       with InhAcc obtain ns3 where Rext3: "Rext' \<omega> \<omega> ns3" and "red_ast_bpl P ctxt (\<gamma>, Normal ns) (?\<gamma>3, Normal ns3)"
         using wf_rel_normal_elim[OF WfInh Rext2] red_ast_bpl_transitive[OF Red2]
         by blast
@@ -230,6 +273,7 @@ proof (rule inhale_rel_intro_2)
         "red_expr_bpl ctxt (mask_upd_bpl (Lang.Var m_bpl) e_rcv_bpl e_f_bpl new_perm_bpl [TConSingle (TNormalFieldId TyRep), \<tau>_bpl])
                            ns3
                            (AbsV (AMask (m ( (r, f_bpl_val) := ?p_bpl))))"
+     *)
        (* 
             from HeapUpdWf have 
             RedHeapUpdBpl:
@@ -247,17 +291,135 @@ proof (rule inhale_rel_intro_2)
            apply (simp add: NewValTypeBpl)
            done
        *)
-        
-        
-      
-    
-    then show ?thesis sorry
   next 
     case InhSubAtomicFailure
-    then show ?thesis sorry
+    hence SubexpFailCases: 
+          "ctxt_vpr, StateCons, Some \<omega> \<turnstile> \<langle>e_rcv_vpr;\<omega>\<rangle> [\<Down>]\<^sub>t VFailure \<or>
+           (\<exists>v. ctxt_vpr, StateCons, Some \<omega> \<turnstile> \<langle>e_rcv_vpr;\<omega>\<rangle> [\<Down>]\<^sub>t (Val v) \<and> 
+                ctxt_vpr, StateCons, Some \<omega> \<turnstile> \<langle>e_p;\<omega>\<rangle> [\<Down>]\<^sub>t VFailure)"
+      by (auto elim: red_exp_list_failure_elim)  
+    show ?thesis
+    proof (rule inhale_rel_aux_intro)
+      show "\<exists>c'. red_ast_bpl P ctxt (\<gamma>, Normal ns) c' \<and> snd c' = Failure"
+      proof (cases "ctxt_vpr, StateCons, Some \<omega> \<turnstile> \<langle>e_rcv_vpr;\<omega>\<rangle> [\<Down>]\<^sub>t VFailure")
+        case True
+        then show ?thesis 
+          using wf_rel_failure_elim[OF WfRcv] \<open>R \<omega> ns\<close>
+          by blast
+      next
+        case False
+        then show ?thesis 
+          using wf_rel_normal_elim[OF WfRcv] \<open>R \<omega> ns\<close> 
+                wf_rel_failure_elim[OF WfPerm] SubexpFailCases red_ast_bpl_transitive
+          by metis
+      qed
+    qed (simp add: \<open>res = _\<close>)
   qed
+qed
+
+definition pred_eq
+  where "pred_eq x v = (x = v)"
+
+lemma pos_perm_rel:
+  assumes ExpRel: "exp_rel_vpr_bpl (state_rel_ext R) ctxt_vpr ctxt e_p e_p_bpl" and
+         DisjAux: "temp_perm \<notin> {heap_var Tr, mask_var Tr} \<union> ran (var_translation Tr) \<union> 
+                     ran (field_translation Tr) \<union> range (const_repr Tr) \<union> dom AuxPred" and
+          StateRel: "\<And> \<omega> ns. R \<omega> ns \<Longrightarrow> state_rel Pr TyRep Tr AuxPred ctxt \<omega> ns" and
+         LookupTyTemp: "lookup_var_ty (var_context ctxt) temp_perm = Some (TPrim TReal)" and
+         WritePermConst: "zero_perm = const_repr Tr CNoPerm"
+
+\<comment>\<open>TODO: handle case where e_p = FullPerm (optimization)\<close>
+  shows "rel_general R
+                  (\<lambda> \<omega> ns.
+                           (\<exists>p. ctxt_vpr, StateCons, Some \<omega> \<turnstile> \<langle>e_p;\<omega>\<rangle> [\<Down>]\<^sub>t Val (VPerm p) \<and>
+                           state_rel Pr TyRep Tr (AuxPred(temp_perm \<mapsto> pred_eq (RealV (real_of_rat p)))) ctxt \<omega> ns))
+                  (\<lambda> \<omega> \<omega>'. \<omega> = \<omega>' \<and> (\<exists>p. ctxt_vpr, StateCons, Some \<omega> \<turnstile> \<langle>e_p;\<omega>\<rangle> [\<Down>]\<^sub>t (Val (VPerm p)) \<and> p \<ge> 0))
+                  (\<lambda> \<omega>. (\<exists>p. ctxt_vpr, StateCons, Some \<omega> \<turnstile> \<langle>e_p;\<omega>\<rangle> [\<Down>]\<^sub>t (Val (VPerm p)) \<and> p < 0))
+                  P ctxt 
+                  ((BigBlock name (Lang.Assign temp_perm e_p_bpl # Assert ((Var temp_perm) \<guillemotleft>Ge\<guillemotright> (Var zero_perm)) # cs) s tr), cont) 
+                  (BigBlock name cs s tr, cont)" (is "rel_general R ?R' ?Success ?Fail  P ctxt ?\<gamma> ?\<gamma>'")
+proof (rule rel_intro)
+  fix \<omega> ns \<omega>'
+  assume "R \<omega> ns" and
+         A: "\<omega> = \<omega>' \<and> (\<exists>p. ctxt_vpr, StateCons, Some \<omega> \<turnstile> \<langle>e_p;\<omega>\<rangle> [\<Down>]\<^sub>t Val (VPerm p) \<and> 0 \<le> p)"
+  from this obtain p
+    where RedPerm: "ctxt_vpr, StateCons, Some \<omega> \<turnstile> \<langle>e_p;\<omega>\<rangle> [\<Down>]\<^sub>t Val (VPerm p)" and "0 \<le> p" 
+    by auto
+
+  note StateRelInst = StateRel[OF \<open>R \<omega> ns\<close>]
+  let ?p_bpl = "real_of_rat p"
+
+  from RedPerm have RedPermBpl: "red_expr_bpl ctxt e_p_bpl ns (RealV ?p_bpl)"
+    using exp_rel_vpr_bpl_elim[OF ExpRel] \<open>R \<omega> ns\<close>
+    by (metis val_rel_vpr_bpl.simps(5))
+
+  let ?ns' = "update_var (var_context ctxt) ns temp_perm (RealV ?p_bpl)"
+
+  have StateRelInst2: "state_rel Pr TyRep Tr (AuxPred(temp_perm \<mapsto> pred_eq (RealV ?p_bpl))) ctxt \<omega> ?ns'"
+    using  state_rel_new_auxvar[OF StateRelInst DisjAux]
+    unfolding pred_eq_def
+    by simp
+
+  moreover have "red_ast_bpl P ctxt
+              (?\<gamma>, Normal ns)
+              ((BigBlock name (Assert ((Var temp_perm) \<guillemotleft>Ge\<guillemotright> (Var zero_perm)) # cs) s tr, cont), Normal ?ns')"
+      (is "red_ast_bpl P ctxt _ (?\<gamma>'',_)")
+    apply (rule red_ast_bpl_one_simple_cmd)
+    by (fastforce intro!: RedAssign LookupTyTemp RedPermBpl)
+
+  moreover have "red_ast_bpl P ctxt (?\<gamma>'', Normal ?ns') (?\<gamma>', Normal ?ns')"
+    apply (rule red_ast_bpl_one_simple_cmd)
+    using \<open>0 \<le> p\<close>
+    by (auto intro!: RedAssertOk Semantics.RedBinOp Semantics.RedVar 
+                        boogie_const_rel_lookup[OF state_rel0_boogie_const[OF state_rel_state_rel0[OF StateRelInst2]]] 
+                simp: \<open>zero_perm = _\<close>)
+
+  ultimately show "\<exists>ns'. red_ast_bpl P ctxt (?\<gamma>, Normal ns) ((BigBlock name cs s tr, cont), Normal ns') \<and>
+                         (\<exists>p. ctxt_vpr, StateCons, Some \<omega>' \<turnstile> \<langle>e_p;\<omega>'\<rangle> [\<Down>]\<^sub>t Val (VPerm p) \<and>
+                              state_rel Pr TyRep Tr (AuxPred(temp_perm \<mapsto> pred_eq (RealV (real_of_rat p)))) ctxt \<omega>' ns')"
+    using RedPerm red_ast_bpl_transitive A
+    by fast
 next
+  fix \<omega> ns
+  assume "R \<omega> ns"
+  assume "\<exists>p. ctxt_vpr, StateCons, Some \<omega> \<turnstile> \<langle>e_p;\<omega>\<rangle> [\<Down>]\<^sub>t Val (VPerm p) \<and> p < 0"
+  from this obtain p
+    where RedPerm: "ctxt_vpr, StateCons, Some \<omega> \<turnstile> \<langle>e_p;\<omega>\<rangle> [\<Down>]\<^sub>t Val (VPerm p)" and "p < 0" 
+    by auto
+
+  note StateRelInst = StateRel[OF \<open>R \<omega> ns\<close>]
+  let ?p_bpl = "real_of_rat p"
+
+  from RedPerm have RedPermBpl: "red_expr_bpl ctxt e_p_bpl ns (RealV ?p_bpl)"
+    using exp_rel_vpr_bpl_elim[OF ExpRel] \<open>R \<omega> ns\<close>
+    by (metis val_rel_vpr_bpl.simps(5))
+
+  let ?ns' = "update_var (var_context ctxt) ns temp_perm (RealV ?p_bpl)"
+
+  have StateRelInst2: "state_rel Pr TyRep Tr (AuxPred(temp_perm \<mapsto> pred_eq (RealV ?p_bpl))) ctxt \<omega> ?ns'"
+    using  state_rel_new_auxvar[OF StateRelInst DisjAux]
+    unfolding pred_eq_def
+    by simp
   
+  moreover have "red_ast_bpl P ctxt
+              (?\<gamma>, Normal ns)
+              ((BigBlock name (Assert ((Var temp_perm) \<guillemotleft>Ge\<guillemotright> (Var zero_perm)) # cs) s tr, cont), Normal ?ns')"
+      (is "red_ast_bpl P ctxt _ (?\<gamma>'',_)")
+    apply (rule red_ast_bpl_one_simple_cmd)
+    by (fastforce intro!: RedAssign LookupTyTemp RedPermBpl)
+
+  moreover have "red_ast_bpl P ctxt (?\<gamma>'', Normal ?ns') (?\<gamma>', Failure)"
+    apply (rule red_ast_bpl_one_simple_cmd)
+    using \<open>p < 0\<close>
+    by (auto intro!: RedAssertFail Semantics.RedBinOp Semantics.RedVar 
+                        boogie_const_rel_lookup[OF state_rel0_boogie_const[OF state_rel_state_rel0[OF StateRelInst2]]] 
+                simp: \<open>zero_perm = _\<close> )
+
+  ultimately show 
+       "\<exists>c'. snd c' = Failure \<and> red_ast_bpl P ctxt (?\<gamma>, Normal ns) c'"
+    using red_ast_bpl_transitive
+    by fastforce
+qed
 
 
 end
